secure_api/merkle_tree/MerkleTree.New.High.fst
@@ -30,7 +30,7 @@ let hash_ss = S.seq hash_seq
 
 noextract
 let hash_init: hash =
-  Seq.create hash_size 0uy
+  Seq.create hash_size (Lib.IntTypes.u8 0)
 
 val hash_2: src1:hash -> src2:hash -> GTot hash
 let hash_2 = MTS.hash2_raw
@@ -65,16 +65,16 @@ private let seq_slice_more_equal #a s1 s2 n m k l =
 /// Facts about "2"
 
 val remainder_2_not_1_div:
-  n:nat -> 
+  n:nat ->
   Lemma (requires (n % 2 <> 1))
         (ensures (n / 2 = (n + 1) / 2))
 let remainder_2_not_1_div n = ()
 
 val remainder_2_1_div:
-  n:nat -> 
+  n:nat ->
   Lemma (requires (n % 2 = 1))
         (ensures (n / 2 + 1 = (n + 1) / 2))
-let remainder_2_1_div n = ()  
+let remainder_2_1_div n = ()
 
 /// High-level Merkle tree data structure
 
@@ -130,7 +130,7 @@ let rec hs_wf_elts_equal lv hs1 hs2 i j =
        S.slice_slice hs2 lv 32 1 (32 - lv);
        assert (S.equal (S.slice hs1 (lv + 1) 32)
 		       (S.slice hs2 (lv + 1) 32));
-       S.lemma_index_slice hs1 lv 32 0; 
+       S.lemma_index_slice hs1 lv 32 0;
        S.lemma_index_slice hs2 lv 32 0;
        assert (S.index hs1 lv == S.index hs2 lv);
        hs_wf_elts_equal (lv + 1) hs1 hs2 (i / 2) (j / 2))
@@ -185,7 +185,7 @@ val insert_:
 let rec insert_ lv i j hs acc =
   let ihs = hash_ss_insert lv i j hs acc in
   assert (S.equal (S.slice hs 0 lv) (S.slice ihs 0 lv));
-  if j % 2 = 1 // S.length (S.index hs lv) > 0 
+  if j % 2 = 1 // S.length (S.index hs lv) > 0
   then begin
     remainder_2_1_div j;
     let nacc = hash_2 (S.last (S.index hs lv)) acc in
@@ -226,7 +226,7 @@ val insert_rec:
 let insert_rec lv i j hs acc = ()
 
 val mt_insert:
-  mt:merkle_tree{mt_wf_elts mt /\ mt_not_full mt} -> v:hash -> 
+  mt:merkle_tree{mt_wf_elts mt /\ mt_not_full mt} -> v:hash ->
   GTot (imt:merkle_tree{mt_wf_elts imt})
 let mt_insert mt v =
   MT (MT?.i mt)
@@ -266,7 +266,7 @@ let rec construct_rhs lv hs rhs i j acc actd =
     (if j % 2 = 0
     then (construct_rhs (lv + 1) hs rhs (i / 2) (j / 2) acc actd)
     else (let nrhs = if actd then S.upd rhs lv acc else rhs in
-         let nacc = if actd 
+         let nacc = if actd
                     then hash_2 (S.index (S.index hs lv) (j - 1 - ofs)) acc
                     else S.index (S.index hs lv) (j - 1 - ofs) in
          construct_rhs (lv + 1) hs nrhs (i / 2) (j / 2) nacc true))
@@ -293,7 +293,7 @@ let rec construct_rhs_unchanged lv hs rhs i j acc actd =
        let rrhs = fst (construct_rhs (lv + 1) hs rhs (i / 2) (j / 2) acc actd) in
        assert (S.equal (S.slice rhs 0 lv) (S.slice rrhs 0 lv)))
   else (let nrhs = if actd then S.upd rhs lv acc else rhs in
-       let nacc = if actd 
+       let nacc = if actd
                   then hash_2 (S.index (S.index hs lv) (j - 1 - ofs)) acc
                   else S.index (S.index hs lv) (j - 1 - ofs) in
        construct_rhs_unchanged (lv + 1) hs nrhs (i / 2) (j / 2) nacc true;
@@ -330,19 +330,19 @@ val construct_rhs_odd:
         (ensures (construct_rhs lv hs rhs i j acc actd ==
                  (let ofs = offset_of i in
                  let nrhs = if actd then S.upd rhs lv acc else rhs in
-                 let nacc = if actd 
+                 let nacc = if actd
                             then hash_2 (S.index (S.index hs lv) (j - 1 - ofs)) acc
                             else S.index (S.index hs lv) (j - 1 - ofs) in
                  construct_rhs (lv + 1) hs nrhs (i / 2) (j / 2) nacc true)))
 let construct_rhs_odd lv hs rhs i j acc actd = ()
 
-val mt_get_root: 
+val mt_get_root:
   mt:merkle_tree{mt_wf_elts mt} -> drt:hash ->
   GTot (merkle_tree * hash)
 let mt_get_root mt drt =
   if MT?.rhs_ok mt then (mt, MT?.mroot mt)
   else begin
-    let (nrhs, rt) = 
+    let (nrhs, rt) =
         construct_rhs
           0 (MT?.hs mt) (MT?.rhs mt) (MT?.i mt) (MT?.j mt)
 	  drt false in
@@ -359,7 +359,7 @@ val mt_get_root_rhs_ok_false:
   mt:merkle_tree{mt_wf_elts mt} -> drt:hash ->
   Lemma (requires (MT?.rhs_ok mt == false))
         (ensures (mt_get_root mt drt ==
-                 (let (nrhs, rt) = 
+                 (let (nrhs, rt) =
                    construct_rhs
                      0 (MT?.hs mt) (MT?.rhs mt) (MT?.i mt) (MT?.j mt)
 	             drt false in
@@ -408,13 +408,13 @@ let mt_get_path_step lv hs rhs i j k p actd =
 		 else p)
 	    else path_insert p (S.index (S.index hs lv) (k + 1 - ofs)))
 
-// Construct a Merkle path for a given index `k`, hashes `hs`, 
+// Construct a Merkle path for a given index `k`, hashes `hs`,
 // and rightmost hashes `rhs`.
 val mt_get_path_:
   lv:nat{lv <= 32} ->
   hs:hash_ss{S.length hs = 32} ->
   rhs:hash_seq{S.length rhs = 32} ->
-  i:nat -> 
+  i:nat ->
   j:nat{
     i <= j /\ j < pow2 (32 - lv) /\
     hs_wf_elts lv hs i j} ->
@@ -435,7 +435,7 @@ val mt_get_path_unchanged:
   lv:nat{lv <= 32} ->
   hs:hash_ss{S.length hs = 32} ->
   rhs:hash_seq{S.length rhs = 32} ->
-  i:nat -> 
+  i:nat ->
   j:nat{
     i <= j /\ j < pow2 (32 - lv) /\
     hs_wf_elts lv hs i j} ->
@@ -459,7 +459,7 @@ val mt_get_path_pull:
   lv:nat{lv <= 32} ->
   hs:hash_ss{S.length hs = 32} ->
   rhs:hash_seq{S.length rhs = 32} ->
-  i:nat -> 
+  i:nat ->
   j:nat{
     i <= j /\ j < pow2 (32 - lv) /\
     hs_wf_elts lv hs i j} ->
@@ -474,7 +474,7 @@ val mt_get_path_pull:
 let rec mt_get_path_pull lv hs rhs i j k p actd =
   let ofs = offset_of i in
   if j = 0 then ()
-  else 
+  else
     (let np = mt_get_path_step lv hs rhs i j k p actd in
     let nactd = if j % 2 = 0 then actd else true in
     mt_get_path_pull (lv + 1) hs rhs (i / 2) (j / 2) (k / 2) np nactd;
@@ -486,7 +486,7 @@ val mt_get_path_slice:
   lv:nat{lv <= 32} ->
   hs:hash_ss{S.length hs = 32} ->
   rhs:hash_seq{S.length rhs = 32} ->
-  i:nat -> 
+  i:nat ->
   j:nat{
     i <= j /\ j < pow2 (32 - lv) /\
     hs_wf_elts lv hs i j} ->
@@ -501,12 +501,12 @@ val mt_get_path_slice:
 let rec mt_get_path_slice lv hs rhs i j k p actd =
   mt_get_path_pull lv hs rhs i j k p actd
 
-val mt_get_path: 
+val mt_get_path:
   mt:merkle_tree{mt_wf_elts mt} ->
   idx:nat{MT?.i mt <= idx /\ idx < MT?.j mt} ->
   drt:hash ->
-  GTot (nat * 
-       (np:path{S.length np = 1 + mt_path_length idx (MT?.j mt) false}) * 
+  GTot (nat *
+       (np:path{S.length np = 1 + mt_path_length idx (MT?.j mt) false}) *
        hash)
 let mt_get_path mt idx drt =
   let (umt, root) = mt_get_root mt drt in
@@ -528,7 +528,7 @@ val mt_flush_to_:
     j >= i /\ j < pow2 (32 - lv) /\
     hs_wf_elts lv hs pi j} ->
   GTot (fhs:hash_ss{
-         S.length fhs = 32 /\ 
+         S.length fhs = 32 /\
          S.equal (S.slice hs 0 lv) (S.slice fhs 0 lv) /\
          hs_wf_elts lv fhs i j}) (decreases i)
 let rec mt_flush_to_ lv hs pi i j =
@@ -558,20 +558,20 @@ val mt_flush_to_rec:
                  let nhs = S.upd hs lv flushed in
                  hs_wf_elts_equal (lv + 1) hs nhs (pi / 2) (j / 2);
                  mt_flush_to_ (lv + 1) nhs (pi / 2) (i / 2) (j / 2))))
-let mt_flush_to_rec lv hs pi i j = ()                 
+let mt_flush_to_rec lv hs pi i j = ()
 
-val mt_flush_to: 
-  mt:merkle_tree{mt_wf_elts mt} -> 
+val mt_flush_to:
+  mt:merkle_tree{mt_wf_elts mt} ->
   idx:nat{idx >= MT?.i mt /\ idx < MT?.j mt} ->
   GTot (fmt:merkle_tree{mt_wf_elts fmt})
 let mt_flush_to mt idx =
   let fhs = mt_flush_to_ 0 (MT?.hs mt) (MT?.i mt) idx (MT?.j mt) in
   MT idx (MT?.j mt) fhs (MT?.rhs_ok mt) (MT?.rhs mt) (MT?.mroot mt)
 
-val mt_flush: 
-  mt:merkle_tree{mt_wf_elts mt /\ MT?.j mt > MT?.i mt} -> 
+val mt_flush:
+  mt:merkle_tree{mt_wf_elts mt /\ MT?.j mt > MT?.i mt} ->
   GTot (fmt:merkle_tree{mt_wf_elts fmt})
-let mt_flush mt = 
+let mt_flush mt =
   mt_flush_to mt (MT?.j mt - 1)
 
 
@@ -582,14 +582,14 @@ val mt_retract_to_:
   lv:nat{lv < S.length hs} ->
   i:nat ->
   s:nat -> // s is the first index excluded from nhs
-  j:nat{ i <= s /\ s <= j /\ 
+  j:nat{ i <= s /\ s <= j /\
          j < pow2 (S.length hs - lv) /\
          hs_wf_elts lv hs i j} ->
   GTot (nhs:hash_ss{
          S.length nhs = S.length hs /\
          S.equal (S.slice hs 0 lv) (S.slice nhs 0 lv) /\
          hs_wf_elts lv nhs i s})
-  (decreases (S.length hs - lv))  
+  (decreases (S.length hs - lv))
 let rec mt_retract_to_ hs lv i s j =
   if lv >= S.length hs then hs
   else begin
@@ -608,14 +608,14 @@ let rec mt_retract_to_ hs lv i s j =
     end
   end
 
-val mt_retract_to: 
-  mt:merkle_tree{mt_wf_elts mt} -> 
+val mt_retract_to:
+  mt:merkle_tree{mt_wf_elts mt} ->
   r:nat{MT?.i mt <= r /\ r < MT?.j mt} ->
   GTot (rmt:merkle_tree{mt_wf_elts rmt /\ MT?.i rmt = MT?.i mt /\ MT?.j rmt = r + 1})
 let mt_retract_to mt r =
-  let nhs = mt_retract_to_ (MT?.hs mt) 0 (MT?.i mt) (r+1) (MT?.j mt) in  
+  let nhs = mt_retract_to_ (MT?.hs mt) 0 (MT?.i mt) (r+1) (MT?.j mt) in
   MT (MT?.i mt) (r+1) nhs false (MT?.rhs mt) (MT?.mroot mt)
-  
+
 
 /// Verification
 
@@ -643,8 +643,7 @@ val mt_verify:
   j:nat{k < j} ->
   p:path{S.length p = 1 + mt_path_length k j false} ->
   rt:hash ->
-  GTot bool
+  GTot prop
 let mt_verify k j p rt =
   let crt = mt_verify_ k j p 1 (S.index p 0) false in
-  crt = rt
-
+  crt == rt
